Entering Coercion Hell

function.lean
@@ -9,20 +9,86 @@ noncomputable theory
 
 set_option pp.beta true
 
-universes u v w
+namespace function
+universes u₁ u₂ u₃ u₄ u₅
+variables {α: Sort u₁} {β: Sort u₂} {γ: Sort u₃} {δ: Sort u₄} {ζ: Sort u₅} --Fixed a bug :P
 
-def comp {α: Sort u} {β: Sort v} {γ: Sort w} (f: β → γ) (g: α → β): α → γ :=
-  λx: α, f (g x)
-instance fun_comp_fun(α: Sort u)(β: Sort v)(γ: Sort w):
-  has_comp (β→γ)(α→β)(α→γ) := @has_comp.mk (β→γ)(α→β)(α→γ) (@comp α β γ)
+@[inline, reducible] def comp (f: β → γ) (g: α → β): α → γ :=
+  λx, f (g x)
 
-constant T: Sort u
-constant U: Sort v
-constant V: Sort w 
+@[inline, reducible] def dcomp {β: α → Sort u₂} {γ: Π{x: α}, β x → Sort u₃}
+  (f: Π{x: α}, Πy: β x, γ y) (g: Πx, β x): Πx, γ (g x) :=
+    λx, f (g x)
 
-constant f: U → V
-constant g: T → U
-constant h: U → U
-#check h
+infixr ` ∘ `:90  := function.comp
+infixr ` ∘' `:80 := function.dcomp
 
--- WIll fix later, have another project in mind
+@[reducible] def comp_right (f: β → β → β) (g: α → β): β → α → β :=
+  λb, λa, f b (g a)
+@[reducible] def comp_left (f: β → β → β) (g: α → β): α → β → β :=
+  λa, λb, f (g a) b
+@[reducible] def on_fun (f: β → β → γ) (g: α → β): α → α → γ :=
+  λx, λy, f (g x) (g y)
+@[reducible] def combine (f: α → β → γ) (op: γ → δ → ζ) (g: α → β → δ): α → β → ζ :=
+  λx, λy, op (f x y) (g x y)
+@[reducible] def const (β: Sort u₂) (a: α): β → α :=
+  λx, a
+@[reducible] def swap {γ: α → β → Sort u₃} (f: Πx, Πy, γ x y): Πy, Πx, γ x y :=
+  λy, λx, f x y
+@[reducible] def app {β: α → Sort u₂} (f: Πx, β x) (x: α): β x :=
+  f x
+
+lemma left_id (f: α → β): id ∘ f = f := eq.refl f
+lemma right_id (f: α → β): f ∘ id = f := eq.refl f
+lemma comp_app (f: β → γ) (g: α → β) (a: α): (f ∘ g) a = f (g a) := eq.refl (f (g a))
+
+lemma comp.assoc (f: γ → δ) (g: β → γ) (h: α → β): (f ∘ g) ∘ h = f ∘ (g ∘ h) := eq.refl (f ∘ (g ∘ h))
+lemma comp.left_id (f: α → β): id ∘ f = f := left_id f
+lemma comp.right_id (f: α → β): f ∘ id = f := right_id f
+
+lemma comp_const_right (f: β → γ) (b: β): f ∘ (const α b) = const α (f b) := eq.refl (const α (f b))
+
+def is_injective(f: α → β) := ∀⦃a₁ a₂: α⦄, f a₁ = f a₂ → a₁=a₂
+def injective(α: Sort u₁)(β: Sort u₂): Sort (max 1 (imax u₁ u₂)) := Σ'f: α → β, is_injective f
+instance Sort_hookrightarrow_Sort: has_hookrightarrow (Sort u₁) (Sort u₂) (Sort (max 1 (imax u₁ u₂))) :=
+  has_hookrightarrow.mk injective
+instance Sort_rightarrowtail_Sort: has_rightarrowtail (Sort u₁) (Sort u₂) (Sort (max 1 (imax u₁ u₂))) :=
+  has_rightarrowtail.mk injective
+instance injective_to_function: has_coe_to_fun (α ↪ β) (λf, α → β) :=
+  has_coe_to_fun.mk (λx: α ↪ β, x.fst)
+lemma injective.comp (g: β ↪ γ) (f: α ↪ β): α ↪ γ :=
+  ⟨(g: β → γ) ∘ (f: α → β),
+  λ⦃a₁ a₂: α⦄, λh, f.snd (g.snd h)⟩ --I want to use `implies.trans` there. I can't!
+infixr (name := inj_comp_inj) ` ∘ `:90  := function.injective.comp
+/- Note to self: You may need more lemmas, the equivalents of `∘`.-/
+def is_surjective(f: α → β) := ∀b: β, ∃a: α, f a = b
+def surjective(α: Sort u₁)(β: Sort u₂): Sort (max 1 (imax u₁ u₂)) := Σ'f: α → β, is_surjective f
+instance Sort_twoheadrightarrow_Sort: has_twoheadrightarrow (Sort u₁) (Sort u₂) (Sort (max 1 (imax u₁ u₂))) :=
+  has_twoheadrightarrow.mk surjective
+instance surjective_to_function: has_coe_to_fun (α ↠ β) (λf, α → β) :=
+  has_coe_to_fun.mk (λx: α ↠ β, x.fst)
+lemma surjective.comp (g: β ↠ γ) (f: α ↠ β): α ↠ γ := 
+  ⟨(g: β→γ)∘(f: α→β), λc: γ, (do
+    let gc: ∃b: β, g b = c := g.snd c,
+    let Fb := λb: β, λgbc: g b = c, (do
+      let fb: ∃a: α, f a = b := f.snd b,
+      let Fa := λa: α, λfab: f a = b, (do
+        let gfa_gb: g (f a) = g b := congr_arg g fab,
+        let gfa_c: g (f a) = c := eq.trans gfa_gb gbc,
+        exists.intro a gfa_c),
+      exists.elim fb Fa),
+    exists.elim gc Fb)⟩
+infixr (name := sur_comp_sur) ` ∘ `:90  := function.surjective.comp
+def is_bijective(f: α → β) := is_injective f ∧ is_surjective f
+def bijective(α: Sort u₁)(β: Sort u₂): Sort (max 1 (imax u₁ u₂)) := Σ'f: α → β, is_bijective f
+instance Sort_twoheadrightarrowtail_Sort: has_twoheadrightarrowtail (Sort u₁) (Sort u₂) (Sort (max 1 (imax u₁ u₂))) :=
+  has_twoheadrightarrowtail.mk bijective
+instance bijective_to_injective: has_coe (α ⤖ β) (α ↪ β) :=
+  has_coe.mk (λf, ⟨f.fst, f.snd.elim_left⟩)
+instance bijective_to_surjective: has_coe (α ⤖ β) (α ↠ β) :=
+  has_coe.mk (λf, ⟨f.fst, f.snd.elim_right⟩)
+instance bijective_to_function: has_coe_to_fun(α ⤖ β) (λf,α → β) :=
+  has_coe_to_fun.mk (λf, f.fst)
+lemma bijective.comp (g: β ⤖ γ) (f: α ⤖ β): α ⤖ γ :=
+  sorry --Blegh, coercion hell
+end function
